code/experimental/pkcs/Hacl.Impl.PKCS11.Session.fst
@@ -7,4 +7,15 @@ open Hacl.Impl.PKCS11.Result
 
 assume val getDeviceInitialised: d: device -> hSession: _CK_SESSION_HANDLE -> Tot bool
 
-assume val sessionVerification: d: device -> hSession: _CK_SESSION_HANDLE -> Tot exception_t
+val sessionVerification: d: device -> hSession: _CK_SESSION_HANDLE -> Tot (e: exception_t
+  {
+    CKR_OK? e <==> getDeviceInitialised d hSession /\
+    CKR_CRYPTOKI_NOT_INITIALIZED? e <==> not (getDeviceInitialised d hSession)
+  }) 
+
+let sessionVerification d hSession = 
+  let deviceInit = getDeviceInitialised d hSession in 
+  if not (deviceInit) then 
+    CKR_CRYPTOKI_NOT_INITIALIZED
+  else
+    CKR_OK
