code/experimental/pkcs/Hacl.Impl.PKCS11.Test.fst
@@ -1,0 +1,33 @@
+module Hacl.Impl.PKCS11.Test
+
+open Hacl.Impl.PKCS11.Creation.GenKey
+
+open Hacl.Impl.PKCS11.Internal.Types
+open Hacl.Impl.PKCS11.Internal.Attribute
+open Hacl.Impl.PKCS11.DeviceModule
+open Hacl.Impl.PKCS11.Session
+
+open Hacl.Impl.PKCS11.Result
+open Hacl.Impl.PKCS11.Parsing
+
+open FStar.HyperStack.All
+open FStar.HyperStack
+module ST = FStar.HyperStack.ST
+
+open Lib.IntTypes
+open LowStar.Buffer
+
+
+val test:   
+  	d: device -> 
+  	hSession: _CK_SESSION_HANDLE -> 
+  	pMechanism: _CK_MECHANISM_TYPE -> 
+  	ulCount: size_t -> 
+  	pTemplate: buffer attributeD {length pTemplate = uint_v ulCount} -> 
+  	Stack (
+    	(exp: exception_t) & (_CK_OBJECT_HANDLE))
+  	(requires fun h -> live h pTemplate)
+  	(ensures fun h0 _ h1 -> True)
+
+
+let test d hSession pMechanism ulCount pTemplate =  _CKS_GenerateKey d hSession pMechanism ulCount pTemplate
